progress on verify proof

proof/correctness/ComputeRootProof.ec
@@ -3,20 +3,61 @@ pragma Goals : printall.
 require import AllCore List RealExp IntDiv Distr DList IntDiv.
 from Jasmin require import JModel JArray.
 
-require import Types Params Parameters Address XMSS_MT_TreeHash.
+require import Types Params Parameters Address WOTS LTree XMSS_MT_TreeHash.
 require import XMSS_IMPL.
 
-require import Array32.
+require import Utils2.
 
-lemma computeRootCorrect : 
+require import Array32 Array64.
+
+op load_nbytes_mem (mem : global_mem_t) (ptr : W64.t) : W8.t Array64.t =
+  Array64.init(fun i => loadW8 mem (to_uint ptr + i)).
+
+(* TODO: Factor out the 8 - end steps of {2} to module root_from_sig_inner *)
+lemma computeRootCorrect (mem : global_mem_t) : 
     equiv [
       M(Syscall).__compute_root ~ RootFromSig.rootFromSig :
-      true 
+      Glob.mem{1} = mem /\
+      Glob.mem{2} = mem /\
+      valid_ptr arg{1}.`4 (W64.of_int 32)
       ==>
       to_list res{1}.`1 = val res{2}
     ].
 proof.
 proc.
+seq 0 8 : (#pre); first by admit.
 seq 2 0 : #pre; first by auto.
+seq 3 0 : (
+  #pre /\
+  auth_path_ptr{1} = _auth_path_ptr{1} /\
+  t32{1} = leaf_idx{1} `&` W32.one 
+); first by auto. 
+seq 1 0 : (
+  #pre /\
+  (t32{1} <> W32.zero => to_list buffer{1} = to_list leaf{1} ++ to_list (load_nbytes_mem mem auth_path_ptr{1}) ) /\
+  (t32{1} = W32.zero  => to_list buffer{1} = to_list (load_nbytes_mem mem auth_path_ptr{1}) ++ to_list leaf{1} )
+).
+    + admit.
+
+seq 1 0 : ( 
+  Glob.mem{1} = mem /\ 
+  Glob.mem{2} = mem /\
+  valid_ptr _auth_path_ptr{1} (of_int 32)%W64 /\
+  to_uint auth_path_ptr{1} = to_uint _auth_path_ptr{1} + 32 /\ 
+  t32{1} = leaf_idx{1} `&` W32.one /\
+  (t32{1} <> W32.zero => to_list buffer{1} = to_list leaf{1} ++ to_list (load_nbytes_mem mem auth_path_ptr{1})) /\
+  (t32{1} = W32.zero => to_list buffer{1} = to_list (load_nbytes_mem mem auth_path_ptr{1}) ++ to_list leaf{1})
+).
+    + auto => /> &1 H0 H1 H2 H3.
+      do split.
+          * admit.
+          * admit.
+          * admit.
+seq 2 2 : #pre.
+
+seq 2 0 : (#pre); last by admit.
+    + admit.
 admit.
+
+
 qed.
