proof/correctness/SignProof.ec
@@ -3,17 +3,20 @@ pragma Goals : printall.
 require import AllCore List RealExp IntDiv Distr DList IntDiv.
 from Jasmin require import JModel JArray.
 
-require import Types Params Parameters Address Notation Hash Primitives Wots XMSS_Commons XMSS_MT_PRF.
+require import Types Params Parameters Address Hash WOTS LTree XMSS_MT_Types XMSS_MT_PRF.
 require import XMSS_IMPL.
 
-require import Repr. 
-require import Util Utils.
+import AuthPath.
+
+
+require import Repr2. 
+require import Utils2.
 
 require import Array4 Array8 Array32 Array64 Array68 Array96 Array132 Array136 Array352 Array2144.
 require import WArray32 WArray96 WArray136.
 
 require import Correctness_Address Correctness_Mem Correctness_Hash.
-require import Utils DistrUtils.
+require import DistrUtils.
 
 require import BitEncoding.
 (*---*) import BitChunking.
@@ -33,13 +36,12 @@ arg{2}.`1 => sk
 arg{2}.`2 => msg
 *)
 
-print mkseq. 
+op load_buf (mem : global_mem_t) (ptr : W64.t) (inlen : W64.t) =
+  mkseq (fun (i : int) => mem.[to_uint ptr + i]) (to_uint inlen).
 
+op max_sig : int = 2 ^ h - 1.
 
-op load_message (mem : global_mem_t) (ptr : W64.t) (mlen : W64.t) =
-  mkseq (fun (i : int) => mem.[to_uint ptr + i]) (to_uint mlen).
-
-
+(* 2500 = XMSS_SIG_BYTES *)
 lemma verify_correct (_sk : W8.t Array132.t, _sm_ptr _smlen_ptr _m_ptr _mlen : W64.t) :
     equiv [
       M(Syscall).__xmssmt_core_sign ~ XMSS_MT_PRF.sign :
@@ -50,22 +52,49 @@ lemma verify_correct (_sk : W8.t Array132.t, _sm_ptr _smlen_ptr _m_ptr _mlen : W
     ].
 proof.
 proc.
-
-swap {2} 5 -4.
-
-seq 12 1 : (
+swap {2} 5 -3.
+seq 12 2 : (
   #pre /\
   exit_0{1} = W8.zero /\
   ots_addr{1} = zero_addr /\
-  address{2} = ots_addr{1}
-); first by inline {1} M(Syscall).__zero_address_; wp; sp; ecall {1} (zero_addr_res addr{1}); skip => />. 
+  idx_new{2} = sk{2}.`Types.idx + W32.one
+).
+    + inline {1} M(Syscall).__zero_address_.
+      wp; sp.
+      ecall {1} (zero_addr_res addr{1}). 
+      skip => />.  
+seq 0 1 : (#pre /\ address{2} = zero_addr).
+    + inline {1} M(Syscall).__zero_address_.
+      auto => />.  
+seq 1 0 : (
+    valid_ptr_i mlen{1} 2500 /\
+    0 <= to_uint sk{2}.`Types.idx &&
+    to_uint sk{2}.`Types.idx < 2 ^ XMSS_FULL_HEIGHT - 1 /\
+    exit_0{1} = W8.zero /\
+    ots_addr{1} = set_type zero_addr 0 /\ 
+    idx_new{2} = sk{2}.`Types.idx + W32.one /\
+    address{2} = zero_addr
+); first by inline {1}; auto => />. 
+seq 0 2 : (
+  #pre /\
+  root{2} = sk{2}.`sk_root /\
+  sk_prf{2} = sk{2}.`Types.sk_prf
+); first by auto.
 
-seq 2 0 : (#pre); first by admit. 
-
-seq 2 0 : (#pre /\ to_uint t64{1} = to_uint mlen{1} + 2500). (* 2500 = XMSS_SIG_BYTES *) 
-    + auto => /> &1 *; rewrite to_uintD of_uintK /#. 
-
-rcondf {1} 3.
-    + admit. 
-
+seq 1 0 : (
+  #pre /\
+  load_buf Glob.mem{1} (sm_ptr{1} + W64.of_int 2500) mlen{1} = load_buf Glob.mem{1} m_ptr{1} mlen{1}
+).
+    + admit.
+seq 2 0 : (#pre /\ t64{1} = mlen{1} + (of_int 2500)%W64); first by auto.
+seq 1 0 : (
+  #pre /\ 
+  loadW64 Glob.mem{1} (to_uint sm_ptr{1}) = t64{1}
+).
+    + auto => /> *.
+      do split. 
+           * admit.
+           * admit.
+swap {2} 2 -1.
+admit.
 qed.
