proof/correctness/VerifyProof.ec
@@ -1,41 +1,99 @@
 pragma Goals : printall.
 
 require import AllCore List RealExp IntDiv Distr DList IntDiv.
+
 from Jasmin require import JModel JArray.
 
-require import Types Params Address XMSS_MT_PRF.
+require import BitEncoding.
+(*---*) import BitChunking.
+
+require import Types Parameters Params Address Hash XMSS_MT_Params XMSS_MT_Types XMSS_MT_TreeHash XMSS_MT_PRF.
 require import XMSS_IMPL.
 
-require import Array32.
+require import Array32 Array64.
 
 require import Correctness_Address.
 
-lemma verify_correct mem :
+require import Repr2.
+
+(*
+  args{1}:
+
+  reg u64 m_ptr mlen_ptr,
+  reg u64 sm_ptr smlen,
+  reg ptr u8[XMSS_PK_BYTES] pk
+
+  returns 0
+*)
+
+(*
+  args{2}
+  pk : xmss_pk
+  m : msg_t
+  s : sig_t
+  
+  returns true
+*)
+
+op load_buf (mem : global_mem_t) (ptr : W64.t) (inlen : W64.t) : W8.t list =
+  mkseq (fun (i : int) => mem.[to_uint ptr + i]) (to_uint inlen).
+
+op sig_size_bytes : int = 2500.
+
+lemma size_bits_to_bytes (x : bool list):
+    size (BitsToBytes x) = size x %/ 8.
+proof.
+rewrite /BitsToBytes size_map size_chunk //.
+qed.
+
+lemma size_lenbytes_be32_4 (x : W32.t) :
+    size (lenbytes_be32 x 4) = 4.
+proof.
+rewrite /lenbytes_be32 size_rev size_take // size_bits_to_bytes size_w2bits //=.
+qed.
+
+lemma load_store_W64 (mem : global_mem_t) (a : address) (v : W64.t) :
+    loadW64 (storeW64 mem a v) a = v.
+proof.
+rewrite /loadW64 pack8E /storeW64. 
+admit.
+qed.
+
+lemma verify_correct (mem : global_mem_t) (mptr mlenptr smptr _smlen : W64.t, pkey : W8.t Array64.t):
+    n = XMSS_N /\
+    d = XMSS_D =>
     equiv[
         M(Syscall).__xmssmt_core_sign_open ~ XMSS_MT_PRF.verify : 
         Glob.mem{1} = mem /\
-        Glob.mem{2} = mem
+        Glob.mem{2} = mem /\
+        arg{1} = (mptr, mlenptr, smptr, _smlen, pkey) /\
+        arg{2}.`1 = EncodePkNoOID pkey /\
+        arg{2}.`2 = load_buf mem mptr (loadW64 mem (to_uint mlenptr))
         ==> 
-        true
-].
+        res{2} <=> res{1} = W64.zero
+    ].
 proof.
+rewrite /XMSS_N /XMSS_D.
+move => [#] n_val d_val. 
 proc.
 seq 9 0 : #pre; first by auto.
-
-seq 1 0 : (#pre /\ to_uint sm_offset{1} = 0); first by auto.
-
-seq 2 0 : (
-  #pre /\
+seq 3 0 : (
+  #pre /\ 
+  to_uint sm_offset{1} = 0 /\
+  to_list pub_root{1} = sub pk{1} 0 32 /\
   to_list pub_seed{1} = val pk{2}.`pk_pub_seed
 ).
-    + auto => /> &1 &2.  
-      admit.
-
-swap {2} 4 -3.
-
-seq 1 0 : (#pre).
-    + auto.
-
+    + auto => />.
+      split.
+          * apply (eq_from_nth witness); [by rewrite size_sub // size_to_list |]. 
+            rewrite size_to_list => j?.             
+            rewrite nth_sub // get_to_list initiE //.
+          * apply (eq_from_nth witness); [by rewrite valP size_to_list n_val |]. 
+            rewrite size_to_list => j?. 
+            rewrite get_to_list initiE // /EncodePkNoOID => />. 
+            rewrite insubdK; [by rewrite /P size_sub // n_val |]. 
+            rewrite nth_sub //. 
+swap {2} 4 -3. 
 seq 1 1 : (
   #pre /\ 
   ots_addr{1} = zero_address /\
@@ -45,7 +103,6 @@ seq 1 1 : (
       wp; sp.
       ecall {1} (zero_addr_res node_addr{1}).
       auto => />. 
-
 seq 1 0 : (
   #pre /\ 
   ltree_addr{1} = zero_address
@@ -54,7 +111,6 @@ seq 1 0 : (
       wp; sp.
       ecall {1} (zero_addr_res ltree_addr{1}).
       auto => />.
-
 seq 1 0 : (
   #pre /\ 
   node_addr{1} = zero_address
@@ -63,5 +119,179 @@ seq 1 0 : (
       wp; sp.
       ecall {1} (zero_addr_res node_addr{1}).
       auto => />.
-admit.
+seq 5 0 : (
+(*  Glob.mem{1} = mem /\
+  Glob.mem{2} = mem /\
+*)
+  m_ptr{1} = mptr /\
+  mlen_ptr{1} = mlenptr /\
+  sm_ptr{1} = smptr /\ 
+  smlen{1} = _smlen /\ 
+  pk{1} = pkey /\
+  pk{2} = EncodePkNoOID pkey /\
+  m{2} = load_buf mem mptr (loadW64 mem (to_uint mlenptr)) /\
+  to_uint sm_offset{1} = 0 /\
+  to_list pub_seed{1} = val pk{2}.`pk_pub_seed /\
+
+  address{2} = zero_address /\
+
+  ots_addr{1} = set_type zero_address 0 /\ 
+  ltree_addr{1} = set_type zero_address 1 /\
+  node_addr{1} = set_type zero_address 2 /\
+  t64{1} = smlen{1} - W64.of_int 2500
+); first by inline; auto => />.
+seq 1 0 : (
+  #pre /\
+  loadW64 Glob.mem{1} (to_uint mlen_ptr{1}) = smlen{1} - W64.of_int 2500
+).
+    + auto => /> &1 *. 
+      by rewrite load_store_W64.
+seq 1 1 : (#pre /\ to_uint idx{1} = to_uint idx_sig{2}).
+    + admit.
+swap {2} 2 -1.
+seq 0 1 : (#pre /\ val seed{2} = sub pk{1} 32 32).
+    + auto => /> &1 &2 ????. 
+      apply (eq_from_nth witness); [by rewrite size_sub // valP n_val |]. 
+      rewrite valP n_val => j?.        
+      rewrite nth_sub // /EncodePkNoOID => />.
+      rewrite insubdK; [by rewrite /P size_sub // n_val |].
+      rewrite nth_sub //.
+
+seq 4 0 : (
+  #pre /\
+  load_buf Glob.mem{1} m_ptr{1} (of_int 2500)%W64 = load_buf Glob.mem{1} sm_ptr{1} (of_int 2500)%W64
+).
+    + admit.
+seq 0 1 : (#pre /\ idx_bytes{2} = lenbytes_be32 idx_sig{2} 4); first by auto.
+
+seq 3 0 : (
+  #pre /\
+  to_list buf{1} = val s{2}.`XMSS_MT_Types.r
+).
+    + admit. (* This requires the operator EncodeSignature *)
+
+seq 0 2 : (
+  #pre /\
+  idx_tree{2} = idx_sig{2} `>>>` h /\
+  idx_leaf{2} = idx_sig{2} `&` (of_int (2^h - 1))%W32
+).
+    + auto =>/> &1 &2 *.
+      rewrite d_val //=.
+seq 2 0 : (
+  m_ptr{1} = mptr /\
+  mlen_ptr{1} = mlenptr /\
+  sm_ptr{1} = smptr /\
+  smlen{1} = _smlen /\
+  pk{1} = pkey /\
+  pk{2} = EncodePkNoOID pkey /\
+  m{2} = load_buf mem mptr (loadW64 mem (to_uint mlenptr)) /\
+  to_uint sm_offset{1} = 0 /\
+  to_list pub_seed{1} = val pk{2}.`pk_pub_seed /\
+  address{2} = zero_address /\
+  ots_addr{1} = set_type zero_address 0 /\
+  ltree_addr{1} = set_type zero_address 1 /\
+  node_addr{1} = set_type zero_address 2 /\
+  loadW64 Glob.mem{1} (to_uint mlen_ptr{1}) =
+  smlen{1} - (of_int 2500)%W64 /\
+  to_uint idx{1} = to_uint idx_sig{2} /\
+  val seed{2} = sub pk{1} 32 32 /\
+  load_buf Glob.mem{1} m_ptr{1} ((of_int 2500))%W64 = load_buf Glob.mem{1} sm_ptr{1} ((of_int 2500))%W64 /\
+  idx_bytes{2} = lenbytes_be32 idx_sig{2} 4 /\
+  to_list buf{1} = val s{2}.`r /\
+  idx_tree{2} = idx_sig{2} `>>>` h /\
+  idx_leaf{2} = idx_sig{2} `&` (of_int (2 ^ h - 1))%W32 /\
+
+  t64{1} = m_ptr{1} + W64.of_int 2372
+); first by auto => />.
+seq 0 3 : (
+  #pre /\ 
+  val root{2} = (sub pk{1} 0 32) /\
+  (sig_ots{2}, auth{2}) = nth witness s{2}.`r_sigs 0 (* first reduced signature *) /\
+  _R{2} = s{2}.`r
+).
+    + auto => /> &1 &2 *. 
+      rewrite /EncodePkNoOID => />; split => [| /#].
+      rewrite insubdK // /P size_sub // n_val //. 
+seq 2 1 : (
+  #pre /\
+  bytes{1} = loadW64 Glob.mem{1} (to_uint mlen_ptr{1}) /\
+  idx_hash{1} = idx{1} /\
+  val t{2} = (val _R{2} ++ val root{2} ++ idx_bytes{2})
+).
+    + auto => /> &1 &2 *.
+      admit.
+seq 1 1 : (#pre /\ to_list root{1} = val _M'{2}). (* This root is the hash of the message *)
+    + admit.
+
+seq 2 0 : (  
+     m_ptr{1} = mptr /\
+     mlen_ptr{1} = mlenptr /\
+     sm_ptr{1} = smptr /\
+     smlen{1} = _smlen /\
+     pk{1} = pkey /\
+     pk{2} = EncodePkNoOID pkey /\
+     m{2} = load_buf mem mptr (loadW64 mem (to_uint mlenptr)) /\
+     to_uint sm_offset{1} =  36 /\
+     to_list pub_seed{1} = val pk{2}.`pk_pub_seed /\
+     address{2} = zero_address /\
+     ots_addr{1} = set_type zero_address 0 /\
+     ltree_addr{1} = set_type zero_address 1 /\
+     node_addr{1} = set_type zero_address 2 /\
+     loadW64 Glob.mem{1} (to_uint mlen_ptr{1}) = smlen{1} - (of_int 2500)%W64 /\
+     to_uint idx{1} = to_uint idx_sig{2} /\
+     val seed{2} = sub pk{1} 32 32 /\
+     load_buf Glob.mem{1} m_ptr{1} ((of_int 2500))%W64 =
+     load_buf Glob.mem{1} sm_ptr{1} ((of_int 2500))%W64 /\
+     idx_bytes{2} = lenbytes_be32 idx_sig{2} 4 /\
+     to_list buf{1} = val s{2}.`r /\
+     idx_tree{2} = idx_sig{2} `>>>` h /\
+     idx_leaf{2} = idx_sig{2} `&` (of_int (2 ^ h - 1))%W32 /\
+    val root{2} = sub pk{1} 0 32 /\
+    (sig_ots{2}, auth{2}) = nth witness s{2}.`r_sigs 0 /\ _R{2} = s{2}.`r /\
+   bytes{1} = loadW64 Glob.mem{1} (to_uint mlen_ptr{1}) /\
+   idx_hash{1} = idx{1} /\
+   val t{2} = val _R{2} ++ val root{2} ++ idx_bytes{2} /\
+  to_list root{1} = val _M'{2}
+).
+    + auto => /> &1 &2 H *.
+      rewrite to_uintD H of_uintK /#.  
+(* handle the results here *)
+seq 2 5 : (
+  pk{2} = EncodePkNoOID pk{1} /\
+  to_list pub_root{1} = sub pk{1} 0 32 /\
+  to_list root{1} = val root{2}
+); last first.
+    + admit.
+seq 0 2 : (
+  m_ptr{1} = mptr /\
+  mlen_ptr{1} = mlenptr /\
+  sm_ptr{1} = smptr /\
+  smlen{1} = _smlen /\
+  pk{1} = pkey /\
+  pk{2} = EncodePkNoOID pkey /\
+  m{2} = load_buf mem mptr (loadW64 mem (to_uint mlenptr)) /\
+  to_uint sm_offset{1} = 36 /\
+  to_list pub_seed{1} = val pk{2}.`pk_pub_seed /\
+  ots_addr{1} = set_type zero_address 0 /\
+  ltree_addr{1} = set_type zero_address 1 /\
+  node_addr{1} = set_type zero_address 2 /\
+  loadW64 Glob.mem{1} (to_uint mlen_ptr{1}) = smlen{1} - (of_int 2500)%W64 /\
+  to_uint idx{1} = to_uint idx_sig{2} /\
+  val seed{2} = sub pk{1} 32 32 /\
+  load_buf Glob.mem{1} m_ptr{1} ((of_int 2500))%W64 =
+  load_buf Glob.mem{1} sm_ptr{1} ((of_int 2500))%W64 /\
+  idx_bytes{2} = lenbytes_be32 idx_sig{2} 4 /\
+  to_list buf{1} = val s{2}.`r /\
+  idx_tree{2} = idx_sig{2} `>>>` h /\
+  idx_leaf{2} = idx_sig{2} `&` (of_int (2 ^ h - 1))%W32 /\
+  val root{2} = sub pk{1} 0 32 /\
+  (sig_ots{2}, auth{2}) = nth witness s{2}.`r_sigs 0 /\
+  _R{2} = s{2}.`r /\
+  bytes{1} = loadW64 Glob.mem{1} (to_uint mlen_ptr{1}) /\
+  idx_hash{1} = idx{1} /\
+  val t{2} = val _R{2} ++ val root{2} ++ idx_bytes{2} /\
+  to_list root{1} = val _M'{2} /\
+
+  address{2} = set_tree_addr (set_layer_addr zero_addr 0) (to_uint idx_tree{2})
+); first by auto => />.
 qed.
