proof/correctness/Properties2.ec
@@ -1,0 +1,64 @@
+pragma Goals : printall.
+
+require import AllCore List RealExp IntDiv.
+
+from Jasmin require import JModel JArray.
+
+require import Params WOTS.
+require import XMSS_IMPL Parameters.
+
+require import Array2 Array3 Array8 Array32 Array64 Array67 Array96 Array2144.
+
+require import Correctness_Mem Correctness_Hash. 
+
+
+require import BitEncoding.
+(*---*) import BitChunking. 
+
+lemma checksum_bounds : 
+    len1 = XMSS_WOTS_LEN1 /\ w = XMSS_WOTS_W =>
+    hoare [
+      WOTS.checksum :
+      size m = 64 /\
+      forall (x : int), x \in m => 0 <= x < w
+      ==>
+      0 <= res <= len1 * (w - 1) 
+    ].
+proof.
+rewrite /XMSS_WOTS_LEN1 /XMSS_WOTS_W => [#] len1_val w_val.
+proc.
+conseq (: 
+  size m = 64 /\
+  forall (k : int), 0 <= k < 64 => 0 <= nth witness m k < 16
+  ==> _
+); first by auto => /> *; smt(@List). 
+while (
+  size m = 64 /\
+  (forall (k : int), 0 <= k < 64 => 0 <= nth witness m k < 16) /\
+  0 <= i <= 64 /\
+  0 <= checksum <= i * (w - 1)
+); first by auto => /> /#. 
+auto => /> &hr ? H0 k j.
+rewrite len1_val w_val //= => H2 H3 H4 H5.
+(have ->: j = 64 by smt()) => /#. 
+qed.
+
+lemma wots_checksum_ll : islossless WOTS.checksum. 
+proof.
+proc.
+while (true) (len1 - i) ; by auto => /> /#.
+qed.
+
+lemma p_checksum_bounds : 
+    len1 = XMSS_WOTS_LEN1 /\ w = XMSS_WOTS_W =>
+    phoare [
+      WOTS.checksum :
+      size m = 64 /\
+      forall (x : int), x \in m => 0 <= x < w
+      ==>
+      0 <= res <= len1 * (w - 1) 
+    ] = 1%r.
+proof.
+move => [#] ??. 
+conseq wots_checksum_ll (checksum_bounds _); [auto | smt() | smt()]. 
+qed.
